LogicalRefinement/Typed/Regular.lean
@@ -207,7 +207,32 @@ theorem HasType.regular (p: Γ ⊢ a: A): A.regular Γ := by {
           exact Hf.upgrade
           exact Hy.upgrade.upgrade
 
-  case prir => sorry
+  case prir Γ A B f x y Hf Hx Hy If Ix Iy => 
+    cases Ix with
+    | expr HA =>
+      cases If with
+      | expr HF =>
+        cases HF with
+        | assume HA HB =>
+          constructor
+          apply HasType.downgrade
+          constructor
+          rw [<-B.subst0_wk1]
+          exact HB.subst0_sort Hx
+          conv =>
+            arg 3
+            rw [<-@Term.subst0_wk1 B x]
+          constructor
+          exact HA.upgrade.assume HB.upgrade
+          exact Hf.upgrade
+          exact Hx.upgrade
+          conv =>
+            arg 3
+            rw [<-@Term.subst0_wk1 B y]
+          constructor
+          exact HA.upgrade.assume HB.upgrade
+          exact Hf.upgrade
+          exact Hy.upgrade
 
   case succ => repeat constructor
 
